trace updates

src/core/DY.Core.Trace.Base.fst
@@ -456,6 +456,33 @@ let state_was_corrupt tr prin sess_id content =
     entry_exists tr (Corrupt time) /\
     entry_at tr time (SetState prin sess_id content)
 
+
+// Reveal label event triggered?
+val reveal_event_triggered_at:
+  #label_t:Type ->
+  trace_ label_t -> timestamp -> principal -> timestamp ->
+  prop
+let reveal_event_triggered_at #label_t tr i prin ts =
+  entry_at tr i (RevealLabel prin ts)
+
+
+val reveal_event_triggered:
+  #label_t:Type ->
+  trace_ label_t -> principal -> timestamp ->
+  prop
+let reveal_event_triggered #label_t tr prin ts =
+  exists i. reveal_event_triggered_at tr i prin ts
+
+val reveal_event_triggered_grows :
+  #label_t:Type ->
+  tr1:trace_ label_t -> tr2:trace_ label_t ->
+  prin:principal -> ts:timestamp ->
+  Lemma
+  (requires reveal_event_triggered tr1 prin ts /\ tr1 <$ tr2)
+  (ensures reveal_event_triggered tr2 prin ts)
+  [SMTPat (reveal_event_triggered tr1 prin ts); SMTPat (tr1 <$ tr2)]
+let reveal_event_triggered_grows tr1 tr2 prin ts = ()
+
 /// Has a (custom, protocol-specific) event been triggered at some timestamp?
 
 val event_triggered_at:
